On remarque que :
\[
  \begin{array}{rrcl}
     & \sum\limits_{n=1}^{\infty}\frac{2}{9n^2-1} & = & \sum\limits_{n=1}^{\infty}\frac{2\times\frac{1}{3}}{n^2-\frac{1}{3}} \\
     &                                            & = & 3 - \psi\left(\frac{1}{3}\right)                                     \\
     &                                            & = & 3 - \pi cotan\left(\frac{\pi}{3}\right)                              \\
     &                                            & = & 3 - \pi \frac{1}{\sqrt{3}}                                           \\
     &                                            & = & 1 - \frac{\pi}{3\sqrt{3}}                                            \\
  \end{array}
\]
D'o√π
\begin{result}
  $\sum\limits_{n=1}^{\infty}\frac{2}{9n^2-1} = 1 - \frac{\pi}{3\sqrt{3}}$
\end{result}
