Soit $t \in \mathbb{R}$.\\
\[
  \left\{
  \begin{array}{rcl}
    x(t) & = & -2cos(t)-cos(2t) \\
    y(t) & = & 2sin(t)-sin(2t)  \\
  \end{array}
  \right.
\]
$x$ et $y$ sont dérivables sur $\mathbb{R}$ en tant que composition de fonctions qui le sont et :

\[
  \left\{
  \begin{array}{rcl}
    x'(t) & = & 2sin(t)+2sin(2t) \\
    y'(t) & = & 2cos(t)-2cos(2t) \\
  \end{array}
  \right.
\]

\[
  \iff
  \left\{
  \begin{array}{rcl}
    x'(t) & = & 2\left[sin(t)+sin(2t)\right]     \\
    y'(t) & = & 2\left[cos(t)-2cos^2(t)+1\right] \\
  \end{array}
  \right.
\]

\[
  \iff
  \left\{
  \begin{array}{rcl}
    x'(t) & = & 2sin(t)\left[1+2cos(t)\right]                        \\
    y'(t) & = & -4\left[cos^2(t)-\frac{1}{2}-\frac{cos(t)}{2}\right] \\
  \end{array}
  \right.
\]

\[
  \iff
  \left\{
  \begin{array}{rcl}
    x'(t) & = & 4sin(t)\left[\frac{1}{2}+cos(t)\right]                      \\
    y'(t) & = & 4\left[-cos^2(t)+\frac{1}{2}+cos(t)-\frac{cos(t)}{2}\right] \\
  \end{array}
  \right.
\]

\[
  \iff
  \left\{
  \begin{array}{rcl}
    x'(t) & = & 4sin(t)\left[\frac{1}{2}+cos(t)\right]                \\
    y'(t) & = & 4\left[1-cos(t)\right]\left[cos(t)+\frac{1}{2}\right] \\
  \end{array}
  \right.
\]
Ainsi on a bien :
\[y'(t) = 4\left[1-cos(t)\right]\left[cos(t)+\frac{1}{2}\right]\]

De plus :
\[
  \begin{array}{crcl}
         & y'(t) & = & 4\left[1-cos(t)\right]\left[cos(t)+\frac{1}{2}\right]                             \\
    \iff & y'(t) & = & 4\left[2
      \left(\underbrace{\frac{1-cos(t)}{2}}_{sin^2\left(\frac{t}{2}\right)}\right)
    \left(\underbrace{\frac{1+cos(t)}{2}}_{cos^2\left(\frac{t}{2}\right)}+\frac{cos(t)}{2}\right)\right] \\
    \iff & y'(t) & = & 4
    \left[
      2\left(sin^2\left(\frac{t}{2}\right)\right)
      \left(cos^2\left(\frac{t}{2}\right)+\frac{cos(t)}{2}\right)
    \right]                                                                                              \\
    \iff & y'(t) & = & 4
    \left[
      2\frac{sin\left(\frac{t}{2}\right)}{cos\left(\frac{t}{2}\right)}
      \left(cos^3\left(\frac{t}{2}\right)sin\left(\frac{t}{2}\right)+\frac{cos(t)}{2}
      \underbrace{cos\left(\frac{t}{2}\right)sin\left(\frac{t}{2}\right)}_{\frac{sin(t)}{2}}
      \right)
    \right]                                                                                              \\
    \iff & y'(t) & = & 4
    \left[
      tan\left(\frac{t}{2}\right)sin(t)
      \left(
      \underbrace{cos^2\left(\frac{t}{2}\right)}_{\frac{1 + cos(t)}{2}}
      + \frac{cos(t)}{2}
      \right)
    \right]                                                                                              \\
    \iff & y'(t) & = &
    tan\left(\frac{t}{2}\right)
    \underbrace{
      4sin(t)
      \left(
      cos(t) + \frac{1}{2}
    \right)}_{x'(t)}                                                                                     \\
    \iff & y'(t) & = & x'(t)tan\left(\frac{t}{2}\right)                                                  \\
  \end{array}
\]
D'où :
\begin{result}
  $
    \left\{
    \begin{array}{rcl}
      y'(t) & = & 4\left[1-cos(t)\right]\left[cos(t)+\frac{1}{2}\right] \\
      y'(t) & = & x'(t)tan\left(\frac{t}{2}\right)                      \\
    \end{array}
    \right.
  $
\end{result}

\begin{flushright}
  CQFD
\end{flushright}
